Z_Operations.thy
@@ -4,25 +4,111 @@ theory Z_Operations
   imports "ITree_UTP.ITree_UTP"
 begin
 
+no_notation (ASCII)
+  Set.member  ("'(:')") and
+  Set.member  ("(_/ : _)" [51, 51] 50) and
+  Set.not_member  ("'(~:')") and
+  Set.not_member  ("(_/ ~: _)" [51, 51] 50)
+
+subsection \<open> Operations \<close>
+
 text \<open> In the most basic form, and operation is simply an indexed Kleisli tree. The index type
   @{typ 'a} represents the inputs and outputs of the operation. \<close>
 
 type_synonym ('e, 'a, 's) operation = "'a \<Rightarrow> ('e, 's) htree"
 
+text \<open> An operation is constructed from a precondition, update, and postcondition, all of which
+  are parameterised. \<close>
+
+definition mk_zop :: "('a \<Rightarrow> 's \<Rightarrow> bool) \<Rightarrow> ('a \<Rightarrow> 's subst) \<Rightarrow> ('a \<Rightarrow> 's \<Rightarrow> bool) \<Rightarrow> ('a \<Rightarrow> ('e, 's) htree)" where
+"mk_zop P \<sigma> Q = (\<lambda> v. assume (P v) ;; assert (Q v) ;; \<langle>\<sigma> v\<rangle>\<^sub>a)"
+
+text \<open> An operation requires that precondition holds, and that following the update the postcondition(s)
+  also hold. \<close>
+
+lemma wp_zop [wp, code_unfold]: "wp (mk_zop P \<sigma> Q v) b = [\<lambda> \<s>. P v \<s> \<and> Q v \<s> \<and> (\<sigma> v \<dagger> [\<lambda> \<s>. b \<s>]\<^sub>e) \<s>]\<^sub>e"
+  by (simp add: mk_zop_def wp)
+
+lemma wlp_zop [wp, code_unfold]: "wlp (mk_zop P \<sigma> Q v) b = [\<lambda> \<s>. P v \<s> \<longrightarrow> Q v \<s> \<longrightarrow> (\<sigma> v \<dagger> [\<lambda> \<s>. b \<s>]\<^sub>e) \<s>]\<^sub>e"
+  by (simp add: mk_zop_def wp)
+
+lemma itree_pre_zop [dpre]: "itree_pre (mk_zop P \<sigma> Q v) = [\<lambda> \<s>. P v \<s>]\<^sub>e"
+  by (simp add: mk_zop_def dpre wp)
+
+lemma itree_rel_zop [itree_rel]: "itree_rel (mk_zop P \<sigma> Q v) = {(x, z). P v x \<and> Q v x \<and> z = \<sigma> v x}"
+  by (simp add: mk_zop_def itree_rel relcomp_unfold)
+
+lemma mk_zop_state_sat: "\<lbrakk> P v s; Q v s \<rbrakk> \<Longrightarrow> mk_zop P \<sigma> Q v s = Ret (\<sigma> v s)"
+  by (simp add: mk_zop_def seq_itree_def kleisli_comp_def assume_def test_def assigns_def)
+
+subsection \<open> Promotion \<close>
+
+text \<open> We implement a promotion scheme where we can extract the local state from a larger
+  global state in order to execute an operation on the former. This requires that we 
+  define a promotion lens. \<close>
+
+definition promotion_lens ::
+  "('ls \<Longrightarrow> 'g) \<comment> \<open> The collection of local states in the global state \<close>
+    \<Rightarrow> ('i \<Rightarrow> 'l \<Longrightarrow> 'ls) \<comment> \<open> An indexed lens for individuals from the collection, (see @{const collection_lens})\<close>
+    \<Rightarrow> 'i \<Rightarrow> 'l \<Longrightarrow> 'g" \<comment> \<open> An indexed lens giving a local state at each index \<close>
+  where
+"promotion_lens x pl = (\<lambda> v. dyn_lens_poly pl x (\<lambda> s. v))"
+
+text \<open> The next gets the set of indices for which a promotion is defined \<close>
+
+definition promotion_type :: "('ls \<Longrightarrow> 'g) \<Rightarrow> ('i \<Rightarrow> 'l \<Longrightarrow> 'ls) \<Rightarrow> 'g \<Rightarrow> \<bbbP> 'i" where
+[expr_defs]: "promotion_type a cl = (\<lambda> s. {i. s \<in> \<S>\<^bsub>cl i ;\<^sub>L a\<^esub>})"
+
+expr_constructor promotion_type
+
+lemma promotion_type_list [simp, code_unfold]: 
+  "vwb_lens a \<Longrightarrow> promotion_type a list_collection_lens = ({0..<length($a)})\<^sub>e"
+  by (simp add: promotion_type_def source_lens_comp source_list_collection_lens wb_lens.source_UNIV, expr_auto)
+
+lemma promotion_type_pfun [simp, code_unfold]:
+  "vwb_lens a \<Longrightarrow> promotion_type a pfun_collection_lens = (dom($a))\<^sub>e"
+  by (simp add: promotion_type_def source_lens_comp source_pfun_collection_lens wb_lens.source_UNIV, expr_simp)
+
+text \<open> Since the set of acceptable parameters of an operation can depend on the state, we need to 
+  lift the type expression as part of the type promotion. \<close>
+
+definition promoted_type :: "('ls \<Longrightarrow> 'g) \<Rightarrow> ('i \<Rightarrow> 'l \<Longrightarrow> 'ls) \<Rightarrow> ('l \<Rightarrow> 'a set) \<Rightarrow> 'g \<Rightarrow> ('i \<times> 'a) set" where
+"promoted_type a cl A = (\<lambda> s. Sigma (promotion_type a cl s) (\<lambda> i. (A \<up> a:cl(i)) s))"
+
+text \<open> The simple case for type promotion is when there is no dependency on the state, as shown
+  below. \<close>
+
+lemma promoted_type_nodep [simp, code_unfold]: 
+  "promoted_type a cl (\<guillemotleft>A\<guillemotright>)\<^sub>e = (promotion_type a cl \<times> \<guillemotleft>A\<guillemotright>)\<^sub>e"
+  by (simp add: promoted_type_def usubst, simp add: SEXP_def)
+
 text \<open> Promoting an operation first checks whether the promotion lens is defined for the given
   index. If not, it deadlocks. Otherwise, the operation is run on the local state, which is
   then injected back into the global state. \<close>
 
-definition promote_op :: "('i \<Rightarrow> ('ls \<Longrightarrow> 's)) \<Rightarrow> ('e, 'a, 'ls) operation \<Rightarrow> ('e, 'i \<times> 'a, 's) operation" where
-"promote_op a P = (\<lambda> (i, v) s. if s \<in> \<S>\<^bsub>a i\<^esub> 
-                               then P v (get\<^bsub>a i\<^esub> s) \<bind> (\<lambda> ls'. Ret (put\<^bsub>a i\<^esub> s ls'))
-                               else deadlock)"
+definition promote_operation :: "('ls \<Longrightarrow> 'g) \<Rightarrow> ('i \<Rightarrow> 'l \<Longrightarrow> 'ls) \<Rightarrow> ('e, 'a, 'l) operation \<Rightarrow> ('e, 'i \<times> 'a, 'g) operation" where
+"promote_operation x pl P = 
+  (let a = promotion_lens x pl
+   in (\<lambda> (i, v) s. P v (get\<^bsub>a i\<^esub> s) \<bind> (\<lambda> ls'. Ret (put\<^bsub>a i\<^esub> s ls'))))"
 
-definition operation :: "('a \<Longrightarrow>\<^sub>\<triangle> 'e) \<Rightarrow> ('e, 'a, 's) operation \<Rightarrow> ('e, 's) htree" where
-"operation c P = c?(v) | pre (P v) \<rightarrow> P v"
+text \<open> The following notation allows us to promote an operation using the inferred collection lens. \<close>
 
-definition io_operation :: "('a \<Longrightarrow>\<^sub>\<triangle> 'e) \<Rightarrow> ('b \<Longrightarrow>\<^sub>\<triangle> 'e) \<Rightarrow> ('a \<Rightarrow> ('e, 'b \<times> 's) htree) \<Rightarrow> ('e, 's) htree" where
-"io_operation c d P = undefined"
+syntax "_promote_op" :: "logic \<Rightarrow> logic \<Rightarrow> logic" ("promote-op")
+translations "_promote_op a P" == "CONST promote_operation a (CONST collection_lens) P"
+
+text \<open> Promotion an operation constructed from a precondition and update requires that we lift
+       the underlying expressions and update. \<close>
+
+lemma promote_mk_zop [wp, code_unfold]:
+  "promote_operation x cl (mk_zop P \<sigma> Q) 
+    = mk_zop 
+        (\<lambda> (a, p). (P p) \<up> x:cl(a)) 
+        (\<lambda> (a, p). (\<sigma> p) \<up>\<^sub>s x:cl(a))
+        (\<lambda> (a, p). (Q p) \<up> x:cl(a))"
+  by (auto simp add: promote_operation_def mk_zop_def Let_unfold promotion_lens_def fun_eq_iff 
+      assume_def seq_itree_def kleisli_comp_def test_def expr_defs assigns_def lens_defs lens_source_def)
+
+subsection \<open> Proof Automation \<close>
 
 method z_wlp uses add = (hoare_wlp_auto add: z_defs add)
 method z_wlp_auto uses add = (hoare_wlp_auto add: z_defs z_locale_defs add)
